src/TwoDisk/AsyncTwoDiskTheorems.v
@@ -82,20 +82,43 @@ Proof.
   eapply disks_rel_stable in H3; eauto.
 Qed.
 
-Theorem covered_stable_pflushed : forall d,
-    Stable (covered d) pflushed.
+Theorem stable_pointwise_rel : forall T T' (d: diskOf T)
+                                 (rel: T -> T' -> Prop)
+                                 (rel': T' -> T' -> Prop),
+    (forall b, Stable (rel b) rel') ->
+    Stable (pointwise_rel rel d) (pointwise_rel rel').
 Proof.
   unfold Stable; intros.
   rename a into d'.
   rename a' into d''.
-  destruct H.
-  inversion H0; subst.
-  econstructor; intros.
+  inversion_clear H0.
+  inversion_clear H1.
+  eapply pointwise_rel_indomain; intros; eauto.
   congruence.
-  specialize (H1 a).
-  simpl_match.
-  destruct (d' a) eqn:?; try contradiction.
-  etransitivity; eauto.
+  specialize (pointwise_rel_holds a).
+  specialize (pointwise_rel_holds0 a).
+  destruct matches in *; eauto; try contradiction.
+Qed.
+
+Theorem collapse_flush : forall h bs bs',
+    collapsesTo h bs ->
+    pflushBlock bs bs' ->
+    collapsesTo h bs'.
+Proof.
+  simpl; intros.
+  inversion H0; subst; clear H0; eauto.
+  destruct H; simpl in *.
+  erewrite curr_val_some_cache in * by eauto.
+  econstructor; simpl; eauto.
+Qed.
+
+Theorem covered_stable_pflush : forall d,
+    Stable (covered d) pflush.
+Proof.
+  intros.
+  eapply stable_pointwise_rel; intros.
+  unfold Stable; intros.
+  eauto using collapse_flush.
 Qed.
 
 Theorem missing_stable : forall A (rel: A -> A -> Prop),
@@ -104,24 +127,25 @@ Proof.
   unfold Stable, missing; eauto.
 Qed.
 
-Hint Resolve covered_stable_pflushed.
+Hint Resolve covered_stable_pflush.
 Hint Resolve missing_stable.
 
-Lemma covered_some_latest : forall (d d': disk) a bs,
+Lemma covered_some_latest : forall (d: histdisk) (d': disk) a bs,
     d' a = Some bs ->
     covered d d' ->
-    d a |= (fun bs' => latest bs' = latest bs).
+    d a |= (fun bs' => curr_val bs' = curr_val bs).
 Proof.
   intros.
+  pose proof (pointwise_rel_holds H0 a).
+  destruct matches in *;
   destruct (d a) eqn:?; eauto.
-  pose proof (covers_pointwise H0 a).
-  simpl.
-  eapply covers_latest_eq; eauto.
+  repeat simpl_match.
+  destruct H1; eauto.
 Qed.
 
 Hint Resolve covered_some_latest.
 
-Lemma covered_none : forall (d d': disk) a F,
+Lemma covered_none : forall (d: histdisk) (d': disk) a F,
     d' a = None ->
     covered d d' ->
     d a |= F.
@@ -129,24 +153,37 @@ Proof.
   intros.
   destruct (d a) eqn:?; eauto.
   exfalso.
-  eauto using same_size_disks_not_different, covered_size_eq.
+  eauto using same_size_disks_not_different, sizes_eq.
 Qed.
 
 Hint Resolve covered_none.
-Hint Resolve then_oldest_oldest.
 
-Theorem disk0_wipe_oldest : forall state F,
+Definition then_wipe (F: disk -> Prop) : disk -> Prop :=
+  fun d' => exists d, F d /\ pflush (wipeDisk d) d'.
+
+Theorem then_wipe_wipe : forall (F: disk -> Prop) d,
+    F d ->
+    then_wipe F (wipeDisk d).
+Proof.
+  unfold then_wipe; intros.
+  descend; intuition eauto.
+  reflexivity.
+Qed.
+
+Hint Resolve then_wipe_wipe.
+
+Theorem disk0_wipe : forall state F,
     TD.disk0 state |= F ->
-    TD.disk0 (TD.wipe state) |= then_oldest F.
+    TD.disk0 (TD.wipe state) |= then_wipe F.
 Proof.
   intros.
   destruct state; simpl in *.
   destruct matches; simpl in *; eauto.
 Qed.
 
-Theorem disk1_wipe_oldest : forall state F,
+Theorem disk1_wipe : forall state F,
     TD.disk1 state |= F ->
-    TD.disk1 (TD.wipe state) |= then_oldest F.
+    TD.disk1 (TD.wipe state) |= then_wipe F.
 Proof.
   intros.
   destruct state; simpl in *.
@@ -161,7 +198,7 @@ Proof.
   firstorder.
 Qed.
 
-Hint Resolve disk0_wipe_oldest disk1_wipe_oldest.
+Hint Resolve disk0_wipe disk1_wipe.
 
 Theorem TDRead0_ok : forall (i: Interface TD.API) a,
     prog_spec
@@ -169,19 +206,19 @@ Theorem TDRead0_ok : forall (i: Interface TD.API) a,
          {|
            pre := TD.disk0 state |= covered d_0 /\
                   TD.disk1 state |= F /\
-                  Stable F pflushed;
+                  Stable F pflush;
            post :=
              fun r state' =>
                match r with
                | Working v => TD.disk0 state' |= covered d_0 /\
                              TD.disk1 state' |= F /\
-                             d_0 a |= (fun bs => latest bs = v)
+                             d_0 a |= (fun bs => curr_val bs = v)
                | Failed => TD.disk0 state' |= missing /\
                           TD.disk1 state' |= F
                end;
            recover :=
-             fun _ state' => TD.disk0 state' |= then_oldest (covered d_0) /\
-                      TD.disk1 state' |= then_oldest F;
+             fun _ state' => TD.disk0 state' |= then_wipe (covered d_0) /\
+                      TD.disk1 state' |= then_wipe F;
          |})
       (Prim i (TD.Read d0 a))
       (irec i)
@@ -189,11 +226,11 @@ Theorem TDRead0_ok : forall (i: Interface TD.API) a,
 Proof.
   prim.
   destruct matches in *; cleanup.
-  eapply disks_rel_stable' in H1; (safe_intuition eauto); cleanup.
-  eapply disks_rel_stable' in H1; (safe_intuition eauto); cleanup.
-  assert (TD.disk0 state'0 |= missing) by eauto.
-  clear H0.
-  eapply disks_rel_stable' in H1; (safe_intuition eauto); cleanup.
+  - eapply disks_rel_stable' in H1; (safe_intuition eauto); cleanup.
+  - eapply disks_rel_stable' in H1; (safe_intuition eauto); cleanup.
+  - assert (TD.disk0 state'0 |= missing) by eauto.
+    clear H0.
+    eapply disks_rel_stable' in H1; (safe_intuition eauto); cleanup.
 Qed.
 
 Theorem TDRead1_ok : forall (i: Interface TD.API) a,
@@ -202,19 +239,19 @@ Theorem TDRead1_ok : forall (i: Interface TD.API) a,
          {|
            pre := TD.disk0 state |= F /\
                   TD.disk1 state |= covered d_1 /\
-                  Stable F pflushed;
+                  Stable F pflush;
            post :=
              fun r state' =>
                match r with
                | Working v => TD.disk0 state' |= F /\
                              TD.disk1 state' |= covered d_1 /\
-                             d_1 a |= (fun bs => latest bs = v)
+                             d_1 a |= (fun bs => curr_val bs = v)
                | Failed => TD.disk0 state' |= F /\
                           TD.disk1 state' |= missing
                end;
            recover :=
-             fun _ state' => TD.disk0 state' |= then_oldest F /\
-                      TD.disk1 state' |= then_oldest (covered d_1);
+             fun _ state' => TD.disk0 state' |= then_wipe F /\
+                      TD.disk1 state' |= then_wipe (covered d_1);
          |})
       (Prim i (TD.Read d1 a))
       (irec i)
@@ -222,27 +259,14 @@ Theorem TDRead1_ok : forall (i: Interface TD.API) a,
 Proof.
   prim.
   destruct matches in *; cleanup.
-  eapply disks_rel_stable' in H1; (safe_intuition eauto); cleanup.
-  eapply disks_rel_stable' in H1; (safe_intuition eauto); cleanup.
-  assert (TD.disk1 state'0 |= missing) by eauto.
-  clear H5.
-  eapply disks_rel_stable' in H1; (safe_intuition eauto); cleanup.
+  - eapply disks_rel_stable' in H1; (safe_intuition eauto); cleanup.
+  - eapply disks_rel_stable' in H1; (safe_intuition eauto); cleanup.
+  - assert (TD.disk1 state'0 |= missing) by eauto.
+    clear H5.
+    eapply disks_rel_stable' in H1; (safe_intuition eauto); cleanup.
 Qed.
 
 (* TODO: move proofs somewhere more appropriate *)
-
-Lemma covers_buffer : forall b bs bs',
-    covers bs bs' ->
-    covers (buffer b bs) (buffer b bs').
-Proof.
-  intros.
-  inversion H; subst; simpl in *.
-  econstructor; intros; eauto.
-  simpl in *; intuition eauto.
-  eapply H0 in H2; intuition eauto.
-Qed.
-
-Hint Resolve covers_buffer.
 
 Lemma covered_diskUpd_buffer : forall d d' a b,
     covered d d' ->
@@ -250,25 +274,23 @@ Lemma covered_diskUpd_buffer : forall d d' a b,
 Proof.
   intros.
   destruct H.
-  econstructor; intros; eauto.
+  eapply pointwise_rel_indomain; intros.
   autorewrite with upd; auto.
-  is_eq a a0; autorewrite with upd in *; eauto.
-  rename a0 into a.
-  destruct (lt_dec a (size d)).
-  - pose proof (@diskUpdF_inbounds _ d a (buffer b) ltac:(auto));
-      repeat deex.
-    assert (a < size d') by congruence.
-    pose proof (@diskUpdF_inbounds _ d' a (buffer b) ltac:(auto));
-      repeat deex.
-    pose proof (covers_pointwise _ _ _ ltac:(eauto) ltac:(eauto)).
+
+  autorewrite with upd in *.
+  assert (a0 < size d') by congruence.
+  specialize (pointwise_rel_holds a0).
+  pose proof (@diskUpdF_inbounds _ d a (buffer b)).
+  pose proof (@diskUpdF_inbounds _ d' a (buffer b)).
+  is_eq a a0;
+    autorewrite with upd in *; destruct matches in *;
+    intuition eauto.
+  repeat deex;
     repeat match goal with
-           | [ H: ?a = Some _,
-                  H': ?a = Some _ |- _ ] =>
-             rewrite H in H'; inversion H'; subst
-           end.
-    eauto.
-  - autorewrite with upd in *.
-    congruence.
+           | [ H: Some _ = Some _ |- _ ] =>
+             inversion H; subst; clear H
+           end; simpl in *.
+  eauto using collapsesTo_buffer.
 Qed.
 
 Hint Resolve covered_diskUpd_buffer.
@@ -279,7 +301,7 @@ Theorem TDWrite0_ok : forall (i: Interface TD.API) a b,
          {|
            pre := TD.disk0 state |= covered d_0 /\
                   TD.disk1 state |= F /\
-                  Stable F pflushed;
+                  Stable F pflush;
            post :=
              fun r state' =>
                match r with
@@ -290,10 +312,10 @@ Theorem TDWrite0_ok : forall (i: Interface TD.API) a b,
                end;
            recover :=
              fun _ state' =>
-               (TD.disk0 state' |= then_oldest (covered d_0) \/
+               (TD.disk0 state' |= then_wipe (covered d_0) \/
                 a < size d_0 /\
-                TD.disk0 state' |= then_oldest (covered (diskUpdF d_0 a (buffer b)))) /\
-               TD.disk1 state' |= then_oldest F;
+                TD.disk0 state' |= then_wipe (covered (diskUpdF d_0 a (buffer b)))) /\
+               TD.disk1 state' |= then_wipe F;
          |})
       (Prim i (TD.Write d0 a b))
       (irec i)
@@ -316,7 +338,7 @@ Theorem TDWrite1_ok : forall (i: Interface TD.API) a b,
          {|
            pre := TD.disk0 state |= F /\
                   TD.disk1 state |= covered d_1 /\
-                  Stable F pflushed;
+                  Stable F pflush;
            post :=
              fun r state' =>
                match r with
@@ -327,10 +349,10 @@ Theorem TDWrite1_ok : forall (i: Interface TD.API) a b,
                end;
            recover :=
              fun _ state' =>
-               TD.disk0 state' |= then_oldest F /\
-               (TD.disk1 state' |= then_oldest (covered d_1) \/
+               TD.disk0 state' |= then_wipe F /\
+               (TD.disk1 state' |= then_wipe (covered d_1) \/
                 a < size d_1 /\
-                TD.disk1 state' |= then_oldest (covered (diskUpdF d_1 a (buffer b))));
+                TD.disk1 state' |= then_wipe (covered (diskUpdF d_1 a (buffer b))));
          |})
       (Prim i (TD.Write d1 a b))
       (irec i)
@@ -352,7 +374,7 @@ Lemma covered_size_eq' : forall d d',
     size d' = size d.
 Proof.
   intros.
-  symmetry; eauto using covered_size_eq.
+  symmetry; eauto using sizes_eq.
 Qed.
 
 Hint Resolve covered_size_eq'.
@@ -363,7 +385,7 @@ Theorem TDDiskSize0_ok : forall (i: Interface TD.API),
          {|
            pre := TD.disk0 state |= covered d_0 /\
                   TD.disk1 state |= F /\
-                  Stable F pflushed;
+                  Stable F pflush;
            post :=
              fun r state' =>
                match r with
@@ -375,8 +397,8 @@ Theorem TDDiskSize0_ok : forall (i: Interface TD.API),
                end;
            recover :=
              fun _ state' =>
-               TD.disk0 state' |= then_oldest (covered d_0) /\
-               TD.disk1 state' |= then_oldest F;
+               TD.disk0 state' |= then_wipe (covered d_0) /\
+               TD.disk1 state' |= then_wipe F;
          |})
       (Prim i (TD.DiskSize d0))
       (irec i)
@@ -394,7 +416,7 @@ Theorem TDDiskSize1_ok : forall (i: Interface TD.API),
          {|
            pre := TD.disk0 state |= F /\
                   TD.disk1 state |= covered d_1 /\
-                  Stable F pflushed;
+                  Stable F pflush;
            post :=
              fun r state' =>
                match r with
@@ -406,8 +428,8 @@ Theorem TDDiskSize1_ok : forall (i: Interface TD.API),
                end;
            recover :=
              fun _ state' =>
-               TD.disk0 state' |= then_oldest F /\
-               TD.disk1 state' |= then_oldest (covered d_1);
+               TD.disk0 state' |= then_wipe F /\
+               TD.disk1 state' |= then_wipe (covered d_1);
          |})
       (Prim i (TD.DiskSize d1))
       (irec i)
@@ -419,38 +441,74 @@ Proof.
   eapply disks_rel_stable' in H1; (safe_intuition eauto); cleanup.
 Qed.
 
+Definition then_flush (F: disk -> Prop) : disk -> Prop :=
+  fun d' => exists d, F d /\ pflush (flush d) d'.
+
 Lemma maybe_holds_then_flush : forall F md d,
     md |= F ->
     md = Some d ->
     then_flush F (flush d).
 Proof.
+  unfold then_flush.
   intros; subst; simpl in *.
-  eauto.
+  exists d; intuition eauto.
+  reflexivity.
 Qed.
 
 Hint Resolve maybe_holds_then_flush.
 
-Lemma stable_then_flush_pflushed : forall F,
-    Stable (then_flush F) pflushed.
+Lemma stable_then_flush_pflush : forall F,
+    Stable (then_flush F) pflush.
 Proof.
   unfold Stable, then_flush; intros.
   repeat deex.
   exists d; intuition.
-  etransitivity; eauto using pflushed_is_covered.
+  etransitivity; eauto.
 Qed.
 
-Hint Resolve stable_then_flush_pflushed.
+Hint Resolve stable_then_flush_pflush.
 
-Theorem then_oldest_then_flush : forall F d,
-    then_oldest (then_flush F) d ->
+Lemma pflush_blockstate_uncached : forall (bs bs': blockstate),
+    cache_val bs = None ->
+    pflush_blockstate bs bs' ->
+    bs = bs'.
+Proof.
+  inversion 2; subst; eauto.
+  congruence.
+Qed.
+
+Lemma wipeBlockstate_cacheval_none : forall bs,
+    cache_val (wipeBlockstate bs) = None.
+Proof.
+  destruct bs; auto.
+Qed.
+
+Hint Resolve wipeBlockstate_cacheval_none.
+
+Theorem then_wipe_then_flush : forall F d,
+    then_wipe (then_flush F) d ->
     then_flush F d.
 Proof.
-  unfold then_oldest, then_flush; intros; repeat deex.
+  unfold then_wipe, then_flush; intros; repeat deex.
   exists d1; intuition.
-  eauto using covered_flush_oldest.
+  destruct H0, H1.
+  eapply pointwise_rel_indomain; intros.
+  etransitivity; eauto.
+  simpl in *.
+  specialize (pointwise_rel_holds a).
+  specialize (pointwise_rel_holds0 a).
+  destruct matches in *; eauto; try contradiction;
+    repeat match goal with
+           | [ H: pflush_blockstate _ _ |- _ ] =>
+             eapply pflush_blockstate_uncached in H;
+               eauto; subst
+           end.
+  unfold wipeBlockstate in *; simpl in *; constructor.
+  destruct b1; simpl in *; subst.
+  unfold wipeBlockstate in *; simpl in *; constructor.
 Qed.
 
-Hint Resolve then_oldest_then_flush.
+Hint Resolve then_wipe_then_flush.
 
 Theorem TDSync0_ok : forall (i: Interface TD.API),
     prog_spec
@@ -458,17 +516,17 @@ Theorem TDSync0_ok : forall (i: Interface TD.API),
          {|
            pre := TD.disk0 state |= F0 /\
                   TD.disk1 state |= F1 /\
-                  Stable F1 pflushed;
+                  Stable F1 pflush;
            post :=
              fun r state' =>
                TD.disk0 state' |= then_flush F0 /\
                TD.disk1 state' |= F1;
            recover :=
              fun _ state' =>
-               (TD.disk0 state' |= then_oldest F0 /\
-                TD.disk1 state' |= then_oldest F1) \/
+               (TD.disk0 state' |= then_wipe F0 /\
+                TD.disk1 state' |= then_wipe F1) \/
                (TD.disk0 state' |= then_flush F0 /\
-                TD.disk1 state' |= then_oldest F1);
+                TD.disk1 state' |= then_wipe F1);
          |})
       (Prim i (TD.Sync d0))
       (irec i)
@@ -488,16 +546,16 @@ Theorem TDSync1_ok : forall (i: Interface TD.API),
          {|
            pre := TD.disk0 state |= F0 /\
                   TD.disk1 state |= F1 /\
-                  Stable F0 pflushed;
+                  Stable F0 pflush;
            post :=
              fun r state' =>
                TD.disk0 state' |= F0 /\
                TD.disk1 state' |= then_flush F1;
            recover :=
              fun _ state' =>
-               (TD.disk0 state' |= then_oldest F0 /\
-                TD.disk1 state' |= then_oldest F1) \/
-               (TD.disk0 state' |= then_oldest F0 /\
+               (TD.disk0 state' |= then_wipe F0 /\
+                TD.disk1 state' |= then_wipe F1) \/
+               (TD.disk0 state' |= then_wipe F0 /\
                 TD.disk1 state' |= then_flush F1);
          |})
       (Prim i (TD.Sync d1))
